fstar/treekem/MLS.TreeKEM.API.Types.fst
@@ -8,7 +8,7 @@ open MLS.TreeKEM.Types
 type treekem_state (bytes:Type0) {|crypto_bytes bytes|} (leaf_ind:nat) = {
   levels: levels:nat{leaf_ind < pow2 levels};
   tree: tree:treekem bytes levels 0{MLS.TreeKEM.Operations.treekem_invariant tree};
-  priv: priv:pathkem_priv bytes levels 0 leaf_ind{MLS.TreeKEM.Operations.treekem_state_invariant tree priv};
+  priv: priv:treekem_priv bytes levels 0 leaf_ind{MLS.TreeKEM.Operations.treekem_state_invariant tree priv};
 }
 
 type treekem_index (#bytes:Type0) {|crypto_bytes bytes|} (#leaf_ind:nat) (st:treekem_state bytes leaf_ind) = i:nat{i < pow2 st.levels}
